\documentclass[11pt,notitlepage]{article}

\usepackage{tikz}
\usetikzlibrary{arrows}
\usetikzlibrary{positioning}
\usetikzlibrary{shapes,shapes.geometric,arrows,fit,calc,positioning,automata,}
\usetikzlibrary{fit,positioning}
\usepackage{lipsum} % Used for inserting dummy 'Lorem ipsum' text into the template
\usepackage{amsfonts, amsmath, amsthm, amssymb} % For math fonts, symbols and environments
\usepackage{graphicx} % Required for including images
\usepackage{booktabs} % Top and bottom rules for table
\usepackage{wrapfig} % Allows in-line images
\usepackage[labelfont=bf]{caption} % Make figure numbering in captions bold
\usepackage[top=0.5in,bottom=0.5in,left=0.5in,right=0.5in]{geometry}


\begin{document}
For the first term of the lower bound equation we have:
\begin{align*}
& \mathbb{E}(\ln Q(\theta)) =\\
& \mathbb{E}(\ln \prod_i Q_i(\theta_i)) =\\
& \mathbb{E}_Q \left( \ln \prod_{n=1}^N \mathcal{N}(X_n|m_x,\Sigma_x)\right) + \mathbb{E}_Q \left( \ln \mathcal{N}(\mathbf{\mu}|\mathbf{m_{\mu}, \mathbf{\Sigma}_x})\right) + \mathbb{E}_Q \left( \ln \prod_{k=1}^d \mathcal{N} (\tilde{w}_k|m_w^{(k)},\Sigma_w)\right)\\
&+ \mathbb{E}_Q \left( \ln \prod_{i=1}^q \Gamma (a_i | \tilde{a}_a, \tilde{b}_{ai})\right) + \mathbb{E}_Q \left( \ln \Gamma (\tau | \tilde{a}_{\tau}, \tilde{b}_{\tau})\right)
\end{align*}
Now, we are going to expand each term of the above equation:
\begin{itemize}
\item 
\begin{align*}
&\mathbb{E}_Q \left( \ln \prod_{n=1}^N \mathcal{N}(X_n|m_x,\Sigma_x)\right) = \\
&\mathbb{E}_Q \left(\sum_{n=1}^N \ln \mathcal{N}(X_n|m_x,\Sigma_x) \right)=\\
&\sum_{n=1}^N \mathbb{E}_Q \left( \ln \left( \left( \cfrac{1}{2\pi}\right)^{q/2} \mathbf{\Sigma_x}^{-1/2} \exp (-\frac{1}{2}(\mathbf{x_n} - \mathbf{m_x})^T \mathbf{\Sigma_x}^{-1}(\mathbf{x_n} - \mathbf{m_x}) )\right) \right)=\\
&\mathbb{E}_Q\left( \cfrac{Nq}{2}\ln \left( \cfrac{1}{2\pi} \right) \right) + \mathbb{E}_Q\left( \cfrac{q}{2} \ln \mathbf{\Sigma_x}  \right) + \mathbb{E}_Q\left( \sum_{n=1}^N (-\frac{1}{2}(\mathbf{x_n} - \mathbf{m_x})^T \mathbf{\Sigma_x}^{-1}(\mathbf{x_n} - \mathbf{m_x})) \right) = \\
&\mathbb{E}_Q\left( \sum_{n=1}^N (-\frac{1}{2}(\mathbf{x_n} - \mathbf{m_x})^T \mathbf{\Sigma_x}^{-1}(\mathbf{x_n} - \mathbf{m_x})) \right) + const = \\
&-\cfrac{1}{2} \sum_{n=1}^N \int Q(x_n) (\mathbf{x_n} - \mathbf{m_x})^T \mathbf{\Sigma_x}^{-1}(\mathbf{x_n} - \mathbf{m_x})\mathrm{d}x_n + const =,\text{ 3.57 Matrix Cookbook}\\
&= \cfrac{N}{2} + Trace(\Sigma_x \Sigma_x^{-1}) + const = \\
&= \cfrac{Nq}{2} +const
\end{align*}
\item 
\begin{equation*}
\mathbb{E}_Q \left( \ln \mathcal{N}(\mathbf{\mu}|\mathbf{m_{\mu}, \mathbf{\Sigma}_x})\right) =  const\text{, similar to the previous derivation.} \\
\end{equation*}
\item
\begin{equation*}
\mathbb{E}_Q \left( \ln \prod_{k=1}^d \mathcal{N} (\tilde{w}_k|m_w^{(k)},\Sigma_w)\right) =  const\text{, similar to the previous two derivations.} \\
\end{equation*}
\item
\begin{align*}
& \mathbb{E}_Q \left( \ln \prod_{i=1}^q \Gamma (a_i | \tilde{a}_a, \tilde{b}_{ai})\right)= \\
& \mathbb{E}_Q\left( \sum_{i=1}^q \ln \Gamma (a_i | \tilde{a}_a, \tilde{b}_{ai}) \right) =\\
& \mathbb{E}_Q\left( \sum_{i=1}^q \ln \left( \cfrac{1}{\Gamma(\tilde{a}_a)} b_{\tilde{a}i}^{\tilde{a}_a} a_i^{\tilde{a}_a -1} e^{-\tilde{b}_{ai}a_i} \right) \right)=\\
& \mathbb{E}_Q\left( \sum_{i=1}^q \left( - \ln\Gamma(\tilde{a}_a) +\ln b_{\tilde{a}i}^{\tilde{a}_a} +\ln a_i^{\tilde{a}_a -1} - \tilde{b}_{ai}a_i  \right) \right)=\\
& -\int \mathrm{d}a_i \sum_{i=1}^q  Q(a_i) \ln\Gamma(\tilde{a}_a) + \int \mathrm{d}a_i \sum_{i=1}^q  Q(a_i) \ln b_{\tilde{a}i}^{\tilde{a}_a} + \int \mathrm{d}a_i \sum_{i=1}^q  Q(a_i) \ln a_i^{\tilde{a}_a -1} - \int \mathrm{d}a_i \sum_{i=1}^q  Q(a_i) \tilde{b}_{ai}a_i =\\
&\text{, in which the first two terms are constants...}\\
&\int \mathrm{d}a_i \sum_{i=1}^q  Q(a_i) \ln a_i^{\tilde{a}_a -1} - \int \mathrm{d}a_i \sum_{i=1}^q  Q(a_i) \tilde{b}_{ai}a_i +const=\\
& (\tilde{a}_a -1)\sum_{i=1}^q \int \mathrm{d}a_i   Q(a_i) \ln a_i - \sum_{i=1}^q \tilde{b}_{ai} \int \mathrm{d}a_i  Q(a_i) a_i +const=\\
&(\tilde{a}_a -1)\sum_{i=1}^q \mathbb{E}_Q[\ln a_i]  - \sum_{i=1}^q \tilde{b}_{ai} \mathbb{E}_Q[a_i]+const  =\\
& (\tilde{a}_a -1)\sum_{i=1}^q \left( \cfrac{\Gamma'(\tilde{a}_a)}{\Gamma(\tilde{a}_a)} - \ln(\tilde{b}_{ai})\right)  - \sum_{i=1}^q \tilde{b}_{ai} \cfrac{\tilde{a}_a}{\tilde{b}_{ai}} +const
\end{align*}
\item
\begin{align*}
&\mathbb{E}_Q \left( \ln \Gamma (\tau | \tilde{a}_{\tau}, \tilde{b}_{\tau})\right) = \\
&\mathbb{E}_Q \left( \ln \left( \cfrac{1}{\Gamma(\tilde{a}_{\tau})} \tilde{b}_{\tau}^{\tilde{a}_{\tau}} \tau^{\tilde{a}_{\tau} -1 } e^{-\tilde{b}_{\tau} \tau} \right) \right) = \\
&\mathbb{E}_Q \left( \ln \cfrac{1}{\Gamma(\tilde{a}_{\tau})} + \ln \tilde{b}_{\tau}^{\tilde{a}_{\tau}}+\ln \tau^{\tilde{a}_{\tau} -1 } + \ln e^{-\tilde{b}_{\tau} \tau} \right) = \\
&\mathbb{E}_Q \left( \ln \cfrac{1}{\Gamma(\tilde{a}_{\tau})} + \ln \tilde{b}_{\tau}^{\tilde{a}_{\tau}}+\ln \tau^{\tilde{a}_{\tau} -1 } -\tilde{b}_{\tau} \tau \right) = \\
& \mathbb{E}_Q \left( \ln \cfrac{1}{\Gamma(\tilde{a}_{\tau})} \right) + \mathbb{E}_Q \left( \ln \tilde{b}_{\tau}^{\tilde{a}_{\tau}} \right) + \mathbb{E}_Q \left( \ln \tau^{\tilde{a}_{\tau} -1 } \right) + \mathbb{E}_Q \left( -\tilde{b}_{\tau} \tau \right) =\\
&\int \mathrm{d}\tau Q(\tau)\ln \cfrac{1}{\Gamma(\tilde{a}_{\tau})}  + \int \mathrm{d}\tau Q(\tau)\ln \tilde{b}_{\tau}^{\tilde{a}_{\tau}}  + \int \mathrm{d}\tau Q(\tau) \ln \tau^{\tilde{a}_{\tau} -1 } + \int \mathrm{d}\tau  Q(\tau) -\tilde{b}_{\tau} \tau=\\
&\text{, in which the first two terms are constants as they are independent of tau.}\\
& \int \mathrm{d}\tau Q(\tau) \ln \tau^{\tilde{a}_{\tau} -1 } + \int \mathrm{d}\tau  Q(\tau) (-\tilde{b}_{\tau} \tau) + const=\\
& (\tilde{a}_{\tau} -1) \int \mathrm{d}\tau Q(\tau) \ln \tau - \tilde{b}_{\tau}\int \mathrm{d}\tau  Q(\tau) \tau+ const=\\
&(\tilde{a}_{\tau} -1) \mathbb{E}_Q(\ln \tau) - \tilde{b}_{\tau} \mathbb{E}_Q(\tau)+ const=\\
&(\tilde{a}_{\tau} -1)\left( \cfrac{\Gamma'(\tilde{a}_{\tau})}{\Gamma(\tilde{a}_{\tau})} - \ln(\tilde{b}_{\tau}) \right) - \tilde{b}_{\tau} \cfrac{\tilde{a}_{\tau}}{\tilde{b}_{\tau}}+ const =\\
&(\tilde{a}_{\tau} -1)\left( \cfrac{\Gamma'(\tilde{a}_{\tau})}{\Gamma(\tilde{a}_{\tau})} - \ln(\tilde{b}_{\tau}) \right) - \tilde{a}_{\tau}+ const
\end{align*}
\end{itemize}
\end{document}